security-monitor/src/core/memory_layout/mod.rs
@@ -1,6 +1,7 @@
 // SPDX-FileCopyrightText: 2023 IBM Corporation
 // SPDX-FileContributor: Wojciech Ozga <woz@zurich.ibm.com>, IBM Research - Zurich
 // SPDX-License-Identifier: Apache-2.0
+#![rr::import("ace.theories.memory_layout", "memory_layout")]
 pub use confidential_memory_address::ConfidentialMemoryAddress;
 pub use confidential_vm_physical_address::ConfidentialVmPhysicalAddress;
 pub use non_confidential_memory_address::NonConfidentialMemoryAddress;
@@ -17,22 +18,27 @@ mod non_confidential_memory_address;
 /// MEMORY_LAYOUT is a static variable (private to this module) that is set during the system boot and never changes
 /// later -- this is guaranteed by Once<>. It stores an instance of the `MemoryLayout`. The only way to get a shared
 /// access to this instance is by calling `MemoryLayout::read()` function.
+#[rr::name("MEMORY_LAYOUT")]
 static MEMORY_LAYOUT: Once<MemoryLayout> = Once::new();
 
 /// Provides an interface to offset addresses that are guaranteed to remain inside the same memory region, i.e.,
 /// confidential or non-confidential memory.
-#[rr::refined_by("(non_conf_start, non_conf_end, conf_start, conf_end)")]
-#[rr::invariant("non_conf_start < non_conf_end")]
-#[rr::invariant("conf_start < conf_end")]
-#[rr::invariant("non_conf_end ≤ conf_start")]
+#[rr::refined_by("ml" : "memory_layout")]
+#[rr::invariant("ml.(non_conf_start).2 ≤ ml.(non_conf_end).2")]
+#[rr::invariant("ml.(conf_start).2 ≤ ml.(conf_end).2")]
+/// Invariant: the non-confidential memory region comes before the confidential memory region.
+#[rr::invariant("ml.(non_conf_end).2 ≤ ml.(conf_start).2")]
+/// Invariant: the bounds of the confidential memory region are aligned to 4KiB pages
+#[rr::invariant("ml.(conf_start) `aligned_to` (page_size_in_bytes_nat Size4KiB)")]
+#[rr::invariant("ml.(conf_end) `aligned_to` (page_size_in_bytes_nat Size4KiB)")]
 pub struct MemoryLayout {
-    #[rr::field("non_conf_start")]
+    #[rr::field("ml.(non_conf_start)")]
     non_confidential_memory_start: *mut usize,
-    #[rr::field("non_conf_end")]
+    #[rr::field("ml.(non_conf_end)")]
     non_confidential_memory_end: *const usize,
-    #[rr::field("conf_start")]
+    #[rr::field("ml.(conf_start)")]
     confidential_memory_start: *mut usize,
-    #[rr::field("conf_end")]
+    #[rr::field("ml.(conf_end)")]
     confidential_memory_end: *const usize,
 }
 
@@ -44,6 +50,7 @@ pub struct MemoryLayout {
 unsafe impl Send for MemoryLayout {}
 unsafe impl Sync for MemoryLayout {}
 
+#[rr::context("onceG Σ memory_layout")]
 impl MemoryLayout {
     const NOT_INITIALIZED_MEMORY_LAYOUT: &'static str = "Bug. Could not access MemoryLayout because is has not been initialized";
 
@@ -54,6 +61,35 @@ impl MemoryLayout {
     /// # Safety
     ///
     /// This function must be called only once by the initialization procedure during the boot of the system.
+    #[rr::skip]
+    #[rr::args("non_conf_start", "non_conf_end", "conf_start", "conf_end")]
+    /// Precondition: The non-confidential memory should have positive size.
+    #[rr::requires("non_conf_start.2 < non_conf_end.2")]
+    /// Precondition: The non-condidential memory should preceed and not overlap with confidential memory.
+    #[rr::requires("non_conf_end.2 ≤ conf_start.2")]
+    /// Precondition: The confidential memory should have positive size.
+    #[rr::requires("conf_start.2 < conf_end.2")]
+    /// Precondition: The global MEMORY_LAYOUT has not been initialized yet.
+    #[rr::requires(#iris "once_initialized π \"MEMORY_LAYOUT\" None")]
+    /// Postcondition: There exists a result -- failure is always an option
+    #[rr::exists("res")]
+    /// Postcondition: failure due to low memory can occur if there is no sufficiently aligned
+    /// confidential address
+    #[rr::ensures("if_err res (λ err, (conf_start.2 - conf_end.2 ≤ page_size_in_bytes_Z Size4KiB)%Z ∧ err = error_Error_Init error_InitType_NotEnoughMemory")]
+    /// Postcondition: if we return Ok, we get a new confidential memory range that is correctly
+    /// aligned for the smallest page size and is a subrange of [conf_start, conf_end)
+    #[rr::ensures(
+        "if_ok res (λ ok, ∃ conf_start' conf_end', conf_start' `aligned_to` (page_size_in_bytes_nat Size4KiB) ∧
+        conf_end' `aligned_to` (page_size_in_bytes_nat Size4KiB) ∧
+        conf_start.2 ≤ conf_start'.2 ∧ conf_end'.2 ≤ conf_end.2 ∧ conf_start'.2 ≤ conf_end'.2 ∧
+        ok = -[ #conf_start'; #conf_end'])%Z"
+    )]
+    /// Postcondition: if we return Ok, the MEMORY_LAYOUT has been initialized.
+    #[rr::ensures(#iris "once_initialized π \"MEMORY_LAYOUT\" (match res with
+        | Ok -[ #conf_start; #conf_end] => Some (mk_memory_layout non_conf_start non_conf_end conf_start conf_end)
+        | _ => None
+        end)")]
+    #[rr::returns("<#>@{result} res")]
     pub unsafe fn init(
         non_confidential_memory_start: *mut usize, non_confidential_memory_end: *const usize, confidential_memory_start: *mut usize,
         mut confidential_memory_end: *const usize,
@@ -90,6 +126,11 @@ impl MemoryLayout {
 
     /// Offsets an address in the confidential memory by a given number of bytes. Returns an error if the resulting
     /// address is not in the confidential memory region.
+    #[rr::only_spec]
+    #[rr::params("bounds", "l", "off")]
+    #[rr::args("#bounds", "#l", "off")]
+    #[rr::requires("l.2 + off < bounds.(conf_end).2")]
+    #[rr::returns("Ok (#(l +ₗ off))")]
     pub fn confidential_address_at_offset(
         &self, address: &ConfidentialMemoryAddress, offset_in_bytes: usize,
     ) -> Result<ConfidentialMemoryAddress, Error> {
@@ -98,6 +139,12 @@ impl MemoryLayout {
 
     /// Offsets an address in the confidential memory by a given number of bytes. Returns an error if the resulting
     /// address is outside the confidential memory region or exceeds the given upper bound.
+    #[rr::only_spec]
+    #[rr::params("bounds", "l", "off", "bound")]
+    #[rr::args("#bounds", "#l", "off", "bound")]
+    #[rr::requires("l.2 + off < bounds.(conf_end).2")]
+    #[rr::requires("bound.2 ≤ bounds.(conf_end).2")]
+    #[rr::returns("Ok (#(l +ₗ off))")]
     pub fn confidential_address_at_offset_bounded(
         &self, address: &ConfidentialMemoryAddress, offset_in_bytes: usize, upper_bound: *const usize,
     ) -> Result<ConfidentialMemoryAddress, Error> {
@@ -107,6 +154,11 @@ impl MemoryLayout {
 
     /// Offsets an address in the non-confidential memory by given number of bytes. Returns an error if the resulting
     /// address is outside the non-confidential memory region.
+    #[rr::only_spec]
+    #[rr::params("bounds", "l", "off")]
+    #[rr::args("#bounds", "#l", "off")]
+    #[rr::requires("l.2 + off < bounds.(non_conf_end).2")]
+    #[rr::returns("Ok (#(l +ₗ off))")]
     pub fn non_confidential_address_at_offset(
         &self, address: &NonConfidentialMemoryAddress, offset_in_bytes: usize,
     ) -> Result<NonConfidentialMemoryAddress, Error> {
@@ -115,6 +167,10 @@ impl MemoryLayout {
     }
 
     /// Returns true if the raw pointer is inside the non-confidential memory.
+    #[rr::only_spec]
+    #[rr::params("bounds", "l")]
+    #[rr::args("#bounds", "l")]
+    #[rr::returns("bool_decide (bounds.(non_conf_start).2 ≤ l.2 ∧ l.2 < bounds.(non_conf_end).2)")]
     pub fn is_in_non_confidential_range(&self, address: *const usize) -> bool {
         self.non_confidential_memory_start as *const usize <= address && address < self.non_confidential_memory_end
     }
@@ -125,6 +181,7 @@ impl MemoryLayout {
     ///
     /// Caller must guarantee that there is no other thread that can write to confidential memory during execution of
     /// this function.
+    // TODO: we need to come up with a mechanism to acquire ownership of all memory
     pub unsafe fn clear_confidential_memory(&self) {
         // We can safely cast the below offset to usize because the constructor guarantees that the confidential memory
         // range is valid, and so the memory size must be a valid usize
@@ -136,13 +193,18 @@ impl MemoryLayout {
         });
     }
 
-    #[rr::skip]
-    #[rr::requires(#iris "initialized_once MEMORY_LAYOUT (non_conf_start, non_conf_end, conf_start, conf_end)")]
-    #[rr::returns("#(non_start, non_end, conf_start, conf_end)")]
+    #[rr::trust_me]
+    #[rr::params("x")]
+    #[rr::requires(#iris "once_initialized π \"MEMORY_LAYOUT\" (Some x)")]
+    #[rr::returns("#x")]
     pub fn read() -> &'static MemoryLayout {
         MEMORY_LAYOUT.get().expect(Self::NOT_INITIALIZED_MEMORY_LAYOUT)
     }
 
+    #[rr::only_spec]
+    #[rr::params("bounds")]
+    #[rr::args("#bounds")]
+    #[rr::returns("-[#bounds.(conf_start).2; #bounds.(conf_end).2]")]
     pub fn confidential_memory_boundary(&self) -> (usize, usize) {
         (self.confidential_memory_start as usize, self.confidential_memory_end as usize)
     }
