security-monitor/src/core/page_allocator/page.rs
@@ -21,29 +21,41 @@ impl PageState for Allocated {}
 
 #[derive(Debug)]
 /// Specification:
-/// Mathematically, we model a `Page` as a triple `(l, sz, v)`, where:
-/// - `l` is the start address in memory,
-/// - `sz` is the size of the page,
-/// - and `v` is the sequence of bytes currently stored in the page.
-#[rr::refined_by("(l, sz, v)" : "loc * page_size * list Z")]
-/// As an invariant, a `Page` *exclusively owns* this memory region, and ascribes the value `v` to it.
-#[rr::invariant(#type "l" : "<#> v" @ "array_t (int usize_t) (page_size_in_words_nat sz)")]
-// TODO: add this once we deal with the Once initialization
-//#[rr::exists("MEMORY_CONFIG")]
-//#[rr::invariant("once_initialized GLOBAL_MEMORY_LAYOUT MEMORY_CONFIG")]
-//#[rr::invariant("page is in range of MEMORY_CONFIG")]
+/// Mathematically, we model a `Page` as a triple `(page_loc, page_sz, page_val)`, where:
+/// - `page_loc` is the start address in memory,
+/// - `page_sz` is the size of the page,
+/// - and `page_val` is the sequence of bytes currently stored in the page.
+#[rr::refined_by("p" : "page")]
+/// Invariant: As an invariant, a `Page` *exclusively owns* this memory region, and ascribes the value `v` to it.
+#[rr::invariant(#type "p.(page_loc)" : "<#> p.(page_val)" @ "array_t (int usize_t) (page_size_in_words_nat p.(page_sz))")]
+/// We require the memory layout to have been initialized.
+#[rr::context("onceG Σ memory_layout")]
+#[rr::exists("MEMORY_CONFIG")]
+/// Invariant: The MEMORY_LAYOUT Once instance has been initialized to MEMORY_CONFIG.
+#[rr::invariant(#iris "once_status \"MEMORY_LAYOUT\" (Some MEMORY_CONFIG)")]
+/// Invariant: ...and according to that layout, this page resides in confidential memory.
+#[rr::invariant("MEMORY_CONFIG.(conf_start).2 ≤ p.(page_loc).2")]
+#[rr::invariant("p.(page_loc).2 + (page_size_in_bytes_nat p.(page_sz)) < MEMORY_CONFIG.(conf_end).2")]
 pub struct Page<S: PageState> {
     /// Specification: the `address` has mathematical value `l`.
-    #[rr::field("l")]
+    #[rr::field("p.(page_loc)")]
     address: ConfidentialMemoryAddress,
     /// Specification: the `size` has mathematical value `sz`.
-    #[rr::field("sz")]
+    #[rr::field("p.(page_sz)")]
     size: PageSize,
     /// Specification: the `_marker` has no relevance for the verification.
     #[rr::field("tt")]
     _marker: PhantomData<S>,
 }
 
+// We declare Send+Sync on the `Page` because it stores internally a raw pointer, which is
+// not safe to pass in a multi-threaded program. But in the case of the `Page` it is safe
+// because the `Page` owns the memory associated with pointer and never exposes the raw pointer
+// to the outside.
+unsafe impl<S> Send for Page<S> where S: PageState {}
+unsafe impl<S> Sync for Page<S> where S: PageState {}
+
+#[rr::context("onceG Σ memory_layout")]
 impl Page<UnAllocated> {
     /// Creates a page token at the given address in the confidential memory.
     ///
@@ -53,26 +65,29 @@ impl Page<UnAllocated> {
     /// and his ownership is given to the page token.
     ///
     /// # Specification:
-    #[rr::params("l", "sz", "v")]
+    #[rr::params("l", "sz", "v", "MEMORY_CONFIG")]
     /// The mathematical values of the two arguments are a memory location `l` and a size `sz`.
     #[rr::args("l", "sz")]
-    /// We require ownership of the memory region starting at `l` for size `sz`.
-    /// Moreover, `l` needs to be properly aligned for a page of size `sz`.
-    /// We view the memory as uninitialized.
+    /// Precondition: We require ownership of the memory region starting at `l` for size `sz`.
+    /// Moreover, `l` needs to be properly aligned for a page of size `sz`, and contain valid integers.
     #[rr::requires(#type "l" : "<#> v" @ "array_t (int usize_t) (page_size_in_words_nat sz)")]
+    /// Precondition: The memory layout is initialized.
+    #[rr::requires(#iris "once_status \"MEMORY_LAYOUT\" (Some MEMORY_CONFIG)")]
+    /// Precondition: The page is entirely contained in the confidential memory range.
+    #[rr::requires("MEMORY_CONFIG.(conf_start).2 ≤ l.2")]
+    #[rr::requires("l.2 + (page_size_in_bytes_nat sz) < MEMORY_CONFIG.(conf_end).2")]
     /// Then, we get a properly initialized page starting at `l` of size `sz` with some value `v`.
-    #[rr::returns("(l, sz, v)")]
+    #[rr::returns("mk_page l sz v")]
     pub(super) unsafe fn init(address: ConfidentialMemoryAddress, size: PageSize) -> Self {
         Self { address, size, _marker: PhantomData }
     }
 
     /// Specification:
     #[rr::skip]
-    #[rr::params("l", "sz", "v")]
-    /// The argument is a page starting at `l` with size `sz` and value `v`.
-    #[rr::args("(l, sz, v)")]
+    #[rr::params("p")]
+    #[rr::args("p")]
     /// We return a page starting at `l` with size `sz`, but with all bytes initialized to zero.
-    #[rr::returns("(l, sz, zero_page sz)")]
+    #[rr::returns("mk_page p.(page_loc) p.(page_sz) (zero_page p.(page_sz))")]
     pub fn zeroize(mut self) -> Page<Allocated> {
         self.clear();
         Page { address: self.address, size: self.size, _marker: PhantomData }
@@ -81,12 +96,21 @@ impl Page<UnAllocated> {
     /// Moves a page to the Allocated state after filling its content with the
     /// content of a page located in the non-confidential memory.
     #[rr::skip]
-    #[rr::params("l" : "loc", "sz", "v", "l2", "v2")]
-    #[rr::args("(l, sz, v)", "l2", "v2")]
-    #[rr::requires(#type "l2" : "v2" @ "value_t (UntypedSynType (mk_page_layout sz))")]
-    #[rr::ensures(#type "l2" : "v2" @ "value_t (UntypedSynType (mk_page_layout sz))")]
-    #[rr::returns("Ok(#(l, sz, v2))")]
+    #[rr::params("p", "l2", "v2", "MEMORY_CONFIG")]
+    #[rr::args("p", "l2", "v2")]
+    /// Precondition: We need to know the current memory layout.
+    #[rr::requires(#iris "once_initialized π \"MEMORY_LAYOUT\" MEMORY_CONFIG")]
+    /// Precondition: The region we are copying from is in non-confidential memory.
+    #[rr::requires("MEMORY_CONFIG.(non_conf_start).2 ≤ l2.2")]
+    #[rr::requires("l2.2 + page_size_in_bytes_Z sz ≤ MEMORY_CONFIG.(non_conf_end).2")]
+    /// Precondition: We require ownership over the memory region.
+    #[rr::requires(#type "l2" : "<#> v2" @ "array_t (int usize_t) (page_size_in_words_nat sz)")]
+    /// Postcondition: We return ownership over the memory region.
+    #[rr::ensures(#type "l2" : "<#> v2" @ "array_t (int usize_t) (page_size_in_words_nat sz)")]
+    #[rr::returns("Ok(#(mk_page p.(page_loc) p.(page_sz) v2))")]
     pub fn copy_from_non_confidential_memory(mut self, mut address: NonConfidentialMemoryAddress) -> Result<Page<Allocated>, Error> {
+        // NOTE: here we get the offsets. We need to prove that the address is still in bounds of non-confidential memory.
+        //
         self.offsets().into_iter().try_for_each(|offset_in_bytes| {
             let non_confidential_address = MemoryLayout::read()
                 .non_confidential_address_at_offset(&mut address, offset_in_bytes)
@@ -103,15 +127,17 @@ impl Page<UnAllocated> {
     /// are correctly aligned. If this page is the smallest page (4KiB for RISC-V), then
     /// the same page is returned.
     #[rr::skip]
-    #[rr::params("MEMORY_CONFIG", "l", "sz", "v")]
-    #[rr::args("(l, sz, v)")]
-    #[rr::requires("once_initialized GLOBAL_MEMORY_LAYOUT MEMORY_CONFIG")]
-    #[rr::returns("subdivide_pages l sz v")]
+    #[rr::params("p", "x")]
+    #[rr::args("p")]
+    /// Precondition: The memory layout needs to have been initialized.
+    #[rr::requires(#iris "initialized π \"MEMORY_LAYOUT\" x")]
+    #[rr::returns("subdivide_pages p.(page_loc) p.(page_sz) p.(page_val)")]
     pub fn divide(mut self) -> Vec<Page<UnAllocated>> {
-        let memory_layout = MemoryLayout::read();
         let smaller_page_size = self.size.smaller().unwrap_or(self.size);
         let number_of_smaller_pages = self.size.in_bytes() / smaller_page_size.in_bytes();
         let page_end = self.end_address_ptr();
+        // NOTE: this needs the invariant to already be open
+        let memory_layout = MemoryLayout::read();
         (0..number_of_smaller_pages)
             .map(|i| {
                 let offset_in_bytes = i * smaller_page_size.in_bytes();
@@ -144,39 +170,41 @@ impl Page<UnAllocated> {
     }
 }
 
+#[rr::context("onceG Σ memory_layout")]
 impl Page<Allocated> {
     /// Clears the entire memory content by writing 0s to it and then converts the Page from Allocated to UnAllocated so it can be returned
     /// to the page allocator.
     #[rr::skip]
-    #[rr::params("l", "sz", "v")]
-    #[rr::args("(l, sz, v)")]
-    #[rr::returns("(l, sz, zero_page sz)")]
+    #[rr::params("p")]
+    #[rr::args("p")]
+    #[rr::returns("mk_page p.(page_loc) p.(page_sz) (zero_page p.(page_sz))")]
     pub fn deallocate(mut self) -> Page<UnAllocated> {
         self.clear();
         Page { address: self.address, size: self.size, _marker: PhantomData }
     }
 }
 
+#[rr::context("onceG Σ memory_layout")]
 impl<T: PageState> Page<T> {
     pub const ENTRY_SIZE: usize = mem::size_of::<usize>();
 
-    #[rr::params("l", "sz", "v")]
-    #[rr::args("#(l, sz, v)")]
-    #[rr::returns("l")]
+    #[rr::params("p")]
+    #[rr::args("#p")]
+    #[rr::returns("p.(page_loc)")]
     pub fn address(&self) -> &ConfidentialMemoryAddress {
         &self.address
     }
 
-    #[rr::params("l", "sz", "v")]
-    #[rr::args("#(l, sz, v)")]
-    #[rr::returns("l.2")]
+    #[rr::params("p")]
+    #[rr::args("#p")]
+    #[rr::returns("p.(page_loc).2")]
     pub fn start_address(&self) -> usize {
         self.address.as_usize()
     }
 
-    #[rr::params("l", "sz", "v")]
-    #[rr::args("#(l, sz, v)")]
-    #[rr::returns("l.2 + page_size_in_bytes_Z sz")]
+    #[rr::params("p")]
+    #[rr::args("#p")]
+    #[rr::returns("p.(page_loc).2 + page_size_in_bytes_Z p.(page_sz)")]
     pub fn end_address(&self) -> usize {
         self.address.as_usize() + self.size.in_bytes()
     }
@@ -191,9 +219,9 @@ impl<T: PageState> Page<T> {
         self.end_address() as *const usize
     }
 
-    #[rr::params("l", "sz", "v")]
-    #[rr::args("#(l, sz, v)")]
-    #[rr::returns("#sz")]
+    #[rr::params("p")]
+    #[rr::args("#p")]
+    #[rr::returns("#(p.(page_sz))")]
     pub fn size(&self) -> &PageSize {
         &self.size
     }
@@ -207,18 +235,18 @@ impl<T: PageState> Page<T> {
     /// will be read from the memory. This offset must be a multiply of size_of::(usize) and be
     /// within the page address range, otherwise an Error is returned.
     /// Specification:
-    #[rr::params("l", "sz", "v", "off")]
-    #[rr::args("#(l, sz, v)", "off")]
+    #[rr::params("p", "off")]
+    #[rr::args("#p", "off")]
     /// Precondition: the offset needs to be divisible by the size of usize.
     #[rr::requires("H_off" : "(ly_size usize_t | off)%Z")]
     /// Precondition: we need to be able to fit a usize at the offset and not exceed the page bounds
-    #[rr::requires("H_sz" : "(off + ly_size usize_t ≤ page_size_in_bytes_Z sz)%Z")]
+    #[rr::requires("H_sz" : "(off + ly_size usize_t ≤ page_size_in_bytes_Z p.(page_sz))%Z")]
     /// Postcondition: there exists some value `x`...
     #[rr::exists("x" : "Z", "off'" : "nat")]
     /// ...where off is a multiple of usize
     #[rr::ensures("(off = off' * ly_size usize_t)%Z")]
     /// ...that has been read from the byte sequence `v` at offset `off`
-    #[rr::ensures("v !! off' = Some x")]
+    #[rr::ensures("p.(page_val) !! off' = Some x")]
     /// ...and we return an Ok containing the value `x`
     #[rr::returns("Ok(#x)")]
     pub fn read(&self, offset_in_bytes: usize) -> Result<usize, Error> {
@@ -245,17 +273,17 @@ impl<T: PageState> Page<T> {
     /// within the page address range, otherwise an Error is returned.
     /// Specification:
     #[rr::trust_me]
-    #[rr::params("l", "sz", "v", "off", "γ", "v2")]
-    #[rr::args("(#(l, sz, v), γ)", "off", "v2")]
+    #[rr::params("p", "off", "γ", "v2")]
+    #[rr::args("(#p, γ)", "off", "v2")]
     /// Precondition: the offset needs to be divisible by the size of usize.
     #[rr::requires("(ly_size usize_t | off)%Z")]
     /// Precondition: we need to be able to fit a usize at the offset and not exceed the page bounds
-    #[rr::requires("(off + ly_size usize_t ≤ page_size_in_bytes_Z sz)%Z")]
+    #[rr::requires("(off + ly_size usize_t ≤ page_size_in_bytes_Z p.(page_sz))%Z")]
     #[rr::exists("off'" : "Z")]
     /// Postcondition: off is a multiple of usize
     #[rr::ensures("off = (off' * ly_size usize_t)%Z")]
     /// Postcondition: self has been updated to contain the value `v2` at offset `off`
-    #[rr::observe("γ": "(l, sz, <[Z.to_nat off' := v2]> v)")]
+    #[rr::observe("γ": "mk_page p.(page_loc) p.(page_sz) (<[Z.to_nat off' := v2]> p.(page_val))")]
     #[rr::returns("Ok(#())")]
     /*
     /// Precondition: the offset needs to be divisible by the size of usize.
@@ -297,9 +325,10 @@ impl<T: PageState> Page<T> {
 
     /// Returns all usize-aligned offsets within the page.
     #[rr::skip]
-    #[rr::args("#(l, sz, v)")]
+    #[rr::params("p")]
+    #[rr::args("#p")]
     // the values that the iterator will yield?
-    #[rr::returns("step_list 0 (ly_size usize_t) (page_size_in_bytes_nat sz)")]
+    #[rr::returns("step_list 0 (ly_size usize_t) (page_size_in_bytes_nat p.(page_sz))")]
     pub fn offsets(&self) -> core::iter::StepBy<Range<usize>> {
         (0..self.size.in_bytes()).step_by(Self::ENTRY_SIZE)
     }
@@ -309,22 +338,20 @@ impl<T: PageState> Page<T> {
     }
 
     #[rr::only_spec]
-    #[rr::params("l", "sz", "v", "γ")]
-    #[rr::args("(#(l, sz, v), γ)")]
-    #[rr::observe("γ": "(l, sz, zero_page sz)")]
+    #[rr::params("p", "γ")]
+    #[rr::args("(#p, γ)")]
+    #[rr::observe("γ": "mk_page p.(page_loc) p.(page_sz) (zero_page p.(page_sz))")]
     fn clear(&mut self) {
         // Safety: below unwrap() is fine because we iterate over page's offsets and thus always
         // request a write to an offset within the page.
         self.offsets().for_each(
             #[rr::skip]
             #[rr::params("off", "v" : "list Z", "l", "sz")]
-
             #[rr::args("off")]
             // this should be dispatched by knowing that each argument is an element of the
             // iterator, i.e. be implied by what for_each can guarantee
             #[rr::requires("(ly_size usize_t | off)%Z")]
             #[rr::requires("(off + ly_size usize_t ≤ page_size_in_bytes_Z sz)%Z")]
-
             #[rr::exists("off'")]
             #[rr::ensures("off = (off' * ly_size usize_t)%Z")]
             #[rr::capture("self" : "(l, sz, v)" -> "(l, sz, <[Z.to_nat off' := 0]> v)")]
