security-monitor/src/core/page_allocator/page_allocator.rs
@@ -1,0 +1,436 @@
+// SPDX-FileCopyrightText: 2023 IBM Corporation
+// SPDX-FileContributor: Wojciech Ozga <woz@zurich.ibm.com>, IBM Research - Zurich
+// SPDX-License-Identifier: Apache-2.0
+#![rr::include("option")]
+#![rr::include("alloc")]
+#![rr::include("btreemap")]
+#![rr::include("vec")]
+#![rr::include("spin")]
+#![rr::import("ace.theories.page_allocator", "page_allocator_extra")]
+use super::page::{Page, UnAllocated};
+use crate::core::memory_layout::{ConfidentialMemoryAddress, MemoryLayout};
+use crate::core::memory_protector::PageSize;
+use crate::error::Error;
+use alloc::collections::BTreeMap;
+use alloc::vec;
+use alloc::vec::Vec;
+use spin::{Once, RwLock, RwLockWriteGuard};
+
+/// Wrappers around BTreeMap operation that use the `Borrow`/`BorrowMut` traits
+/// (which RefinedRust doesn't support well)
+mod btreemap {
+    use alloc::collections::BTreeMap;
+
+    #[rr::only_spec]
+    #[rr::context("EqDecision {rt_of K}")]
+    #[rr::context("Countable {rt_of K}")]
+    #[rr::params("m", "k")]
+    #[rr::args("#m", "#k")]
+    #[rr::returns("<#>@{option} (m !! k)")]
+    pub fn btr_get<'a, 'b, K, V>(m: &'a BTreeMap<K, V>, key: &'b K) -> Option<&'a V>
+    where K: Ord {
+        m.get(key)
+    }
+
+    #[rr::only_spec]
+    #[rr::context("EqDecision {rt_of K}")]
+    #[rr::context("Countable {rt_of K}")]
+    #[rr::params("m", "k", "γ")]
+    #[rr::args("(#m, γ)", "#k")]
+    #[rr::exists("γi")]
+    #[rr::returns("if decide (is_Some (m !! k)) then Some (#(m !!! k, γi)) else None")]
+    #[rr::observe("γ": "if decide (is_Some (m !! k)) then <[k := PlaceGhost γi]> m else m")]
+    pub fn btr_get_mut<'a, 'b, K, V>(m: &'a mut BTreeMap<K, V>, key: &'b K) -> Option<&'a mut V>
+    where K: Ord {
+        m.get_mut(key)
+    }
+}
+
+/// A static global structure containing unallocated pages. Once<> guarantees that the PageAllocator can only be initialized once.
+#[rr::name("PAGE_ALLOCATOR")]
+static PAGE_ALLOCATOR: Once<RwLock<PageAllocator>> = Once::new();
+
+/// The `PageAllocator`'s job is to pass ownership of free pages residing in the confidential memory. It guarantees that a physical page is
+/// not allocated twice. It does so by giving away `Page` tokens that represent ownership of a physical page located in the confidental
+/// memory as described by `MemoryLayout`. `PageAllocator`'s constructor creates page tokens (maintaining an invariant that there are no two
+/// page tokens describing the same physical address).
+/// Specification:
+/// We model the memory tracker by a finite map assigning page sizes to the number of available pages.
+#[rr::refined_by("map" : "gmap page_size nat")]
+/// Internally, the tracker stores a map with more information, containing the full model of the pages.
+#[rr::exists("page_map")]
+/// Invariant: This map is related by containing the number of pages as specified by `m`.
+#[rr::invariant("page_allocator_maps_related map page_map")]
+/// Invariant: The internal map should have a vector of pages for every page size.
+#[rr::invariant("∀ k : page_size, is_Some (map !! k)")]
+#[rr::context("onceG Σ memory_layout")]
+pub struct PageAllocator {
+    #[rr::field("page_map")]
+    map: BTreeMap<PageSize, Vec<Page<UnAllocated>>>,
+}
+
+#[rr::context("onceG Σ memory_layout")]
+#[rr::context("onceG Σ unit")]
+impl<'a> PageAllocator {
+    // Usually there are 512 pages of size x that can fit in a single page of size y, where y is next page size larger than x (e.g., 2MiB
+    // and 4KiB).
+    const EXPECTED_NUMBER_OF_TOKENS_PER_SIZE: usize = 512;
+    const NOT_INITIALIZED: &'static str = "Bug. Could not access page allocator because it is not initialized";
+
+    /// Initializes the global instance of a `PageAllocator`. Returns error if the `PageAllocator` has already been initialized.
+    ///
+    /// # Arguments
+    ///
+    /// See the `PageAllocator::add_memory_region` for requirements on arguments.
+    ///
+    /// # Safety
+    ///
+    /// See the `PageAllocator::add_memory_region` for safety requirements.
+    #[rr::only_spec]
+    #[rr::params("conf_start", "conf_end", "vs")]
+    #[rr::args("conf_start", "conf_end")]
+    /// Precondition: The start address needs to be aligned to the minimum page size.
+    #[rr::requires("Hstart_aligned" : "conf_start `aligned_to` (page_size_in_bytes_nat Size4KiB)")]
+    /// Precondition: The minimum page size divides the memory size.
+    #[rr::requires("Hsz_div" : "(page_size_in_bytes_nat Size4KiB) | (conf_end.2 - conf_start.2)")]
+    /// Precondition: The memory range should not be negative.
+    #[rr::requires("Hstart_lt" : "conf_start.2 ≤ conf_end.2")]
+    /// Precondition: We have ownership of the memory range, having (conf_end - conf_start) bytes.
+    #[rr::requires(#type "conf_start" : "vs" @ "array_t (int u8) (Z.to_nat (conf_end.2 - conf_start.2))")]
+    /// Precondition: The page allocator should be uninitialized.
+    #[rr::requires(#iris "once_initialized π \"PAGE_ALLOCATOR\" None")]
+    /// Postcondition: The page allocator is initialized.
+    #[rr::ensures(#iris "once_initialized π \"PAGE_ALLOCATOR\" (Some ())")]
+    /// TODO: require this to be in confidential memory?
+    #[rr::returns("Ok(#())")]
+    pub unsafe fn initialize(memory_start: ConfidentialMemoryAddress, memory_end: *const usize) -> Result<(), Error> {
+        assure_not!(PAGE_ALLOCATOR.is_completed(), Error::Reinitialization())?;
+        let mut page_allocator = Self::empty();
+        page_allocator.add_memory_region(memory_start, memory_end);
+        PAGE_ALLOCATOR.call_once(|| RwLock::new(page_allocator));
+        Ok(())
+    }
+
+    /// Constructs an empty page allocator that contains no tokens.
+    ///
+    /// # Guarantees
+    ///
+    /// * The PageAllocator's map contains keys for every possible page size.
+    #[rr::only_spec]
+    #[rr::exists("m")]
+    #[rr::returns("m")]
+    fn empty() -> Self {
+        let mut map = BTreeMap::new();
+        for page_size in PageSize::all_from_largest_to_smallest() {
+            let page_tokens = Vec::<_>::with_capacity(Self::EXPECTED_NUMBER_OF_TOKENS_PER_SIZE);
+            map.insert(page_size.clone(), page_tokens);
+        }
+        Self { map }
+    }
+
+    /// Adds a physial memory region to the PageAllocator. The ownership over this memory region is passed from the caller to the
+    /// PageAllocator. This function constructs page tokens over this memory region and stores them in the PageAllocator.
+    ///
+    /// # Arguments
+    ///
+    /// `memory_region_start` address must be aligned to the smallest page size and lower than `memory_region_end`.
+    /// `memory_region_end` address must be aligned to the smallest page size. This address is one-past-the end of the memory region whose
+    /// ownership is given to the `PageAllocator`.
+    ///
+    /// # Guarantees
+    ///
+    /// * There are no two page tokens that describe the same memory address.
+    ///
+    /// # Safety
+    ///
+    /// The caller must guarantee that he passes the ownership to the memory region described by the input arguments to the PageAllocator.
+    #[rr::only_spec]
+    #[rr::params("mstart", "mend", "m", "γ", "vs", "MEMORY_CONFIG")]
+    #[rr::args("(#m, γ)", "mstart", "mend")]
+    /// Precondition: The start address needs to be aligned to the minimum page size.
+    #[rr::requires("Hstart_aligned" : "mstart `aligned_to` (page_size_in_bytes_nat Size4KiB)")]
+    /// Precondition: The minimum page size divides the memory size.
+    #[rr::requires("Hsz_div" : "(page_size_in_bytes_nat Size4KiB) | (mend.2 - mstart.2)")]
+    /// Precondition: The memory range is positive.
+    #[rr::requires("Hstart_lt" : "mstart.2 < mend.2")]
+    /// Precondition: We have ownership of the memory range, having (mend - mstart) bytes.
+    #[rr::requires(#type "mstart" : "vs" @ "array_t (int u8) (Z.to_nat (mend.2 - mstart.2))")]
+    /// Precondition: The memory layout needs to be initialized
+    #[rr::requires(#iris "once_initialized π \"MEMORY_LAYOUT\" (Some MEMORY_CONFIG)")]
+    /// Precondition: the whole memory region should be part of confidential memory
+    /// TODO: should we require this or silently drop memory if it's outside the range?
+    /// Postcondition: There exists some correctly initialized page assignment.
+    #[rr::exists("m'" : "gmap page_size nat")]
+    #[rr::observe("γ": "m'")]
+    unsafe fn add_memory_region(&mut self, memory_region_start: ConfidentialMemoryAddress, memory_region_end: *const usize) {
+        debug!("Memory tracker: adding memory region: 0x{:x} - 0x{:x}", memory_region_start.as_usize(), memory_region_end as usize);
+        assert!(memory_region_start.is_aligned_to(PageSize::smallest().in_bytes()));
+        assert!(memory_region_end.is_aligned_to(PageSize::smallest().in_bytes()));
+        assert!(memory_region_start.as_usize() < memory_region_end as usize);
+
+        // Our strategy is to create as few page tokens as possible to keep the memory overhead as low as possible. Therefore, we prefer to
+        // create page tokens for the largest page size when possible. We use a greedy approach. We look for the largest possible page that
+        // can be accomodated for the given address and create a page token for it. We start with the smallest possible page size and then
+        // keep increasing it until we find the largest possible page size. Then, we keep decreasing the page size until we reach the end of
+        // the memory region.
+        let memory_layout = MemoryLayout::read();
+        let mut memory_address = Some(memory_region_start);
+        let mut page_size = PageSize::smallest();
+
+        // We might have to create a few tokens of 4KiB until we reach the address at which we can fit a 2MiB page. Then, we might have to
+        // create a few tokens for 2MiB pages until we get the address where 1 GiB page would fit. Consider the following example,
+        // where we first create 7x 4 KiB tokens (++), then 3x 2 MiB tokens (**), and only then start creating 1 GiB tokens (##).
+        //
+        //      ++ ++ ++ ++ ++ ++ ++  ***********************  ***********************  ***********************  ####
+        // ||  |  |  |  |  |  |  |  ||  |  |  |  |  |  |  |  ||  |  |  |  |  |  |  |  ||  |  |  |  |  |  |  |  || ...
+        //     ^memory_region_start  ^2 MiB                   ^2 MiB                   ^2 MiB                   ^1GiB
+        //
+        // At certain point we will not be able to fit more page tokens of the highest size (1GiB in our example) because remaining space
+        // will be lower than the used page size. We might, however, still fit tokens of smaller sizes. This will be a analogous (but
+        // opposite) situation to the one presented above. According to the following example, we will fit 3x 2 MiB (**) and 4x 4 KiB (++)
+        // page tokens to the remaining memory region.
+        //
+        //   ***********************  ***********************  ***********************  ++ ++ ++ ++
+        // ||  |  |  |  |  |  |  |  ||  |  |  |  |  |  |  |  ||  |  |  |  |  |  |  |  ||  |  |  |  |  |  |  |  || ...
+        //  ^1 GiB                   ^2 MiB                   ^2 MiB                   ^2 MiB      ^memory_region_end
+
+        // According to the RISC-V spec, pages must be aligned to their size.
+        let is_address_page_aligned =
+            |address: &ConfidentialMemoryAddress, page_size: &PageSize| address.is_aligned_to(page_size.in_bytes());
+        // Page can be created only if all bytes are belonging to the given memory region
+        let can_create_page = |address: &ConfidentialMemoryAddress, page_size: &PageSize| {
+            let page_last_address = page_size.in_bytes() - 1;
+            memory_layout.confidential_address_at_offset_bounded(&address, page_last_address, memory_region_end).is_ok()
+        };
+
+        while let Some(address) = memory_address.take() {
+            // Let's find the largest possible size of a page that could align to this address.
+            while let Some(larger_size) = page_size.larger().filter(|larger_size| is_address_page_aligned(&address, &larger_size)) {
+                page_size = larger_size;
+            }
+            // Now let's find the largest size of a page that really fits in the given memory region. We do not have to check the alignment,
+            // because the larger pages sizes are multiplies of the smaller page sizes.
+            while let Some(smaller_size) = page_size.smaller().filter(|smaller_size| !can_create_page(&address, &smaller_size)) {
+                page_size = smaller_size;
+            }
+            // The following line ensures that the while loop will complete because, regardless of whether we manage to create a page token
+            // or not, we will increment the `memory_address` in each loop so that it eventually passes the end of the given memory region.
+            memory_address = memory_layout.confidential_address_at_offset_bounded(&address, page_size.in_bytes(), memory_region_end).ok();
+            // If the next memory address (`memory_address`) is still in the memory range, then we are sure we can create the page token.
+            // Otherwise, we must check the boundary condition: Are we creating the last page token over a memory whose last byte
+            // (`address`+`page_size.in_bytes()`) is next to the end of the memory region (`memory_region_end`)?
+            if memory_address.is_some() || can_create_page(&address, &page_size) {
+                let new_page_token = Page::<UnAllocated>::init(address, page_size.clone());
+                // Below unwrap is safe because the PageAllocator constructor guarantees the initialization of the map for all possible page
+                // sizes.
+                btreemap::btr_get_mut(&mut self.map, &page_size).unwrap().push(new_page_token);
+            }
+        }
+
+        self.map.iter().for_each(|(page_size, tokens)| {
+            debug!("Created {} page tokens of size {:?}", tokens.len(), page_size);
+        })
+    }
+
+    /// Returns page tokens that all together have ownership over a continous unallocated memory region of the requested size. Returns error
+    /// if it could not obtain write access to the global instance of the page allocator or if there are not enough page tokens satisfying
+    /// the requested criteria.
+    #[rr::only_spec]
+    #[rr::params("num", "sz")]
+    #[rr::args("num", "sz")]
+    /// Precondition: The page allocator needs to be initialized.
+    #[rr::requires(#iris "once_initialized π \"PAGE_ALLOCATOR\" (Some ())")]
+    /// Postcondition: there exists a result (the error case is always a valid option)
+    #[rr::exists("res")]
+    /// Postcondition: errors are always a valid outcome
+    #[rr::ensures("if_Err res (λ err, err = error_Error_OutOfMemory)")]
+    /// Postcondition: if sucessful, we get the desired number of pages of the right size
+    #[rr::ensures("if_Ok res (λ pages, Z.of_nat (length pages) = num ∧ (∀ x, x ∈ pages → ∃ p, x = #p ∧ p.(page_sz) = sz))")]
+    #[rr::returns("<#>@{result} res")]
+    pub fn acquire_continous_pages(number_of_pages: usize, page_size: PageSize) -> Result<Vec<Page<UnAllocated>>, Error> {
+        let pages = Self::try_write(|page_allocator| Ok(page_allocator.acquire(number_of_pages, page_size)))?;
+        assure_not!(pages.is_empty(), Error::OutOfPages())?;
+        Ok(pages)
+    }
+
+    /// Consumes the page tokens given by the caller, allowing for their further acquisition. This is equivalent to deallocation of the
+    /// physical memory region owned by the returned page tokens.
+    ///
+    /// TODO: to prevent fragmentation, run a procedure that will try to combine page tokens of smaller sizes into page tokens of bigger
+    /// sizes. Otherwise, after long run, the security monitor's might start occupying to much memory (due to large number of page tokens)
+    /// and being slow.
+    #[rr::only_spec]
+    #[rr::params("pages")]
+    #[rr::args("pages")]
+    /// Precondition: We require the page allocator to be initialized.
+    #[rr::requires(#iris "once_initialized π \"PAGE_ALLOCATOR\" (Some ())")]
+    pub fn release_pages(pages: Vec<Page<UnAllocated>>) {
+        let _ = Self::try_write(|page_allocator| {
+            Ok(pages.into_iter().for_each(
+                #[rr::skip]
+                #[rr::params("m" : "gmap page_size nat", "p")]
+                #[rr::capture("page_allocator" : "m" -> "<[p.(page_sz) := 1 + m !!! p.(page_sz)]> m")]
+                #[rr::args("p")]
+                |page| {
+                    let mut pg = &mut *page_allocator;
+                    btreemap::btr_get_mut(&mut pg.map, &page.size()).and_then(|v| Some(v.push(page)));
+                },
+            ))
+        })
+        .inspect_err(
+            #[rr::only_spec]
+            #[rr::params("x")]
+            #[rr::args("x")]
+            |_| debug!("Memory leak: failed to store released pages in the page allocator"),
+        );
+    }
+
+    #[rr::trust_me]
+    #[rr::params("p")]
+    #[rr::args("p")]
+    /// Precondition: We require the page allocator to be initialized.
+    #[rr::requires(#iris "once_initialized π \"PAGE_ALLOCATOR\" (Some ())")]
+    pub fn release_page(page: Page<UnAllocated>) {
+        let mut pages = Vec::with_capacity(1);
+        pages.push(page);
+        Self::release_pages(pages)
+    }
+
+    /// Returns vector of unallocated page tokens representing a continous memory region. If it failes to find allocation within free pages
+    /// of the requested size, it divides larger page tokens. Empty vector is returned if there are not enough page tokens in the system
+    /// that meet the requested criteria.
+    // NOTE: this has the same specification as `acquire_continuous_pages_of_given_size`
+    #[rr::only_spec]
+    #[rr::params("m", "γ", "num", "sz")]
+    #[rr::args("(#m, γ)", "num", "sz")]
+    /// Precondition: We require the page allocator to be initialized.
+    #[rr::requires(#iris "once_initialized π \"PAGE_ALLOCATOR\" (Some ())")]
+    #[rr::exists("pages", "m'" : "gmap page_size nat")]
+    /// Postcondition: If pages are available in the current PageAllocator, then we return them.
+    #[rr::ensures("if decide (num ≤ Z.of_nat (m !!! sz))%Z then Z.of_nat (length pages) = num else Z.of_nat (length pages) = 0")]
+    /// Postcondition: The returned pages have the appropriate size
+    #[rr::ensures("∀ p i, pages !! i = Some p → p.(page_sz) = sz")]
+    /// Postcondition: The pages are continuous
+    #[rr::ensures("pages_are_contiguous pages")]
+    /// Postcondition: The map has been updated.
+    #[rr::observe("γ": "m'")]
+    #[rr::returns("<#> pages")]
+    fn acquire(&mut self, number_of_pages: usize, page_size: PageSize) -> Vec<Page<UnAllocated>> {
+        let mut available_pages = self.acquire_continous_pages_of_given_size(number_of_pages, page_size);
+        // it might be that there is not enough page tokens of the requested page size. In such a case, let's try to divide page tokens of
+        // larger page sizes and try the allocation again.
+        if available_pages.is_empty() {
+            self.divide_pages(page_size);
+            available_pages = self.acquire_continous_pages_of_given_size(number_of_pages, page_size);
+        }
+        available_pages
+    }
+
+    /// Tries to allocate a continous chunk of physical memory composed of the requested number of pages. Returns a vector of unallocated
+    /// page tokens, all of them having the same size, or an empty vector if the allocation fails.
+    #[rr::only_spec]
+    #[rr::params("m", "γ", "num", "sz")]
+    #[rr::args("(#m, γ)", "num", "sz")]
+    /// Precondition: We require the page allocator to be initialized.
+    #[rr::requires(#iris "once_initialized π \"PAGE_ALLOCATOR\" (Some ())")]
+    #[rr::exists("pages", "m'" : "gmap page_size nat")]
+    /// Postcondition: If pages are available in the current PageAllocator, then we return them.
+    #[rr::ensures("if decide (num ≤ Z.of_nat (m !!! sz))%Z then Z.of_nat (length pages) = num else Z.of_nat (length pages) = 0")]
+    /// Postcondition: The returned pages have the appropriate size
+    #[rr::ensures("∀ p i, pages !! i = Some p → p.(page_sz) = sz")]
+    /// Postcondition: The pages are continuous
+    #[rr::ensures("pages_are_contiguous pages")]
+    /// Postcondition: The map has been updated.
+    #[rr::observe("γ": "m'")]
+    #[rr::returns("<#> pages")]
+    fn acquire_continous_pages_of_given_size(&mut self, number_of_pages: usize, page_size: PageSize) -> Vec<Page<UnAllocated>> {
+        // Below unwrap is safe because the PageAllocator constructor guarantees that the map contains keys for every possible page size.
+        let pages = btreemap::btr_get_mut(&mut self.map, &page_size).unwrap();
+        if pages.len() < number_of_pages {
+            // early return because there is not enough page tokens for the requested page size.
+            return vec![];
+        }
+
+        // Checks if consecutive pages at the given range compose a continuous memory region. The assumption is that pages are sorted.
+        // Thus, it is enough to check if all neighbouring page tokens compose a continuous memory region.
+        let is_memory_region_continous = |pages: &mut Vec<Page<UnAllocated>>, start_index: usize, end_index: usize| {
+            (start_index..(end_index - 1)).all(|page_index| pages[page_index].end_address() == pages[page_index + 1].start_address())
+        };
+
+        let mut allocated_pages = Vec::with_capacity(number_of_pages);
+        let last_possible_index = pages.len() - number_of_pages;
+        (0..last_possible_index)
+            .find(|&allocation_start_index| {
+                let allocation_end_index = allocation_start_index + number_of_pages;
+                is_memory_region_continous(pages, allocation_start_index, allocation_end_index)
+            })
+            .inspect(|allocation_start_index| {
+                // we found allocation, lets return page tokens to the caller
+                (0..number_of_pages).for_each(|_| {
+                    // `Vec::push` appends to the end of the vector, so we preserve the order of pages. `Vec::remove` removes the page token
+                    // at the given index and shifts left all other page tokens, so we preserve the order of pages in the map
+                    allocated_pages.push(pages.remove(*allocation_start_index))
+                })
+            });
+        allocated_pages
+    }
+
+    /// Tries to divide existing page tokens, so that the PageAllocator has page tokens of the requested page size.
+    #[rr::only_spec]
+    #[rr::params("m", "γ", "sz")]
+    #[rr::args("(#m, γ)", "sz")]
+    #[rr::exists("m'" : "gmap page_size nat")]
+    /// Postcondition: the page size division has been updated
+    #[rr::observe("γ": "m'")]
+    fn divide_pages(&mut self, page_size: PageSize) {
+        let mut page_size_to_divide_next = page_size.larger();
+        while let Some(page_size_to_divide_now) = page_size_to_divide_next {
+            if page_size_to_divide_now == page_size {
+                break;
+            }
+            if self.divide_page(page_size_to_divide_now) {
+                // as soon as we manage to find and divide a larger page token, we start to to iterate back over smaller page sizes and
+                // divide them into even smaller page tokens. Eventually, we end up with the requested page_size that will exit the while
+                // loop.
+                page_size_to_divide_next = page_size_to_divide_now.smaller();
+            } else {
+                // in the case when there are no more page tokens in the system, the page_size_to_divide becomes eventually None and
+                // exits the while loop.
+                page_size_to_divide_next = page_size_to_divide_now.larger();
+            }
+        }
+    }
+
+    /// Tries to divide a page of the given size into smaller pages. Returns false if there is no page of the given size or the given size
+    /// is the smallest possible page size supported by the architecture.
+    #[rr::only_spec]
+    #[rr::params("m", "γ", "sz")]
+    #[rr::args("(#m, γ)", "sz")]
+    #[rr::exists("success", "m'")]
+    /// Postcondition: the page size division has been updated
+    #[rr::observe("γ": "m'")]
+    /// Postcondition: if the division was successful, then sufficient pages at the requested size available
+    #[rr::ensures("if success then (m' !!! default Size4KiB (page_size_smaller sz)) ≥ 256 else m' = m")]
+    #[rr::returns("success")]
+    fn divide_page(&mut self, from_size: PageSize) -> bool {
+        from_size
+            .smaller()
+            .and_then(|to_size| {
+                // Below unwraps are safe because the PageAllocator constructor guarantees that the map contains keys for every possible
+                // page size.
+                btreemap::btr_get_mut(&mut self.map, &from_size).unwrap().pop().and_then(|page| {
+                    btreemap::btr_get_mut(&mut self.map, &to_size).unwrap().append(&mut page.divide());
+                    Some(true)
+                })
+            })
+            .unwrap_or(false)
+    }
+
+    /// returns a mutable reference to the PageAllocator after obtaining a lock on the mutex
+    #[rr::skip]
+    // TODO: might be challenging to specify
+    fn try_write<F, O>(op: O) -> Result<F, Error>
+    where O: FnOnce(&mut RwLockWriteGuard<'static, PageAllocator>) -> Result<F, Error> {
+        op(&mut PAGE_ALLOCATOR.get().expect(Self::NOT_INITIALIZED).write())
+    }
+}
