verification/generated_code/ace/proofs/proof_core_memory_layout_MemoryLayout_read.v
@@ -1,17 +1,21 @@
 From caesium Require Import lang notation.
 From refinedrust Require Import typing shims.
 From sm.ace.generated Require Import generated_code_ace generated_specs_ace.
-From sm.ace.generated Require Import generated_template_core_memory_layout_confidential_memory_address_ConfidentialMemoryAddress_new.
+From sm.ace.generated Require Import generated_template_core_memory_layout_MemoryLayout_read.
 
 Set Default Proof Using "Type".
 
 Section proof.
 Context `{!refinedrustGS Σ}.
-Lemma core_memory_layout_confidential_memory_address_ConfidentialMemoryAddress_new_proof (π : thread_id) :
-  core_memory_layout_confidential_memory_address_ConfidentialMemoryAddress_new_lemma π.
-Proof.
-  core_memory_layout_confidential_memory_address_ConfidentialMemoryAddress_new_prelude.
 
+Lemma core_memory_layout_MemoryLayout_read_proof (π : thread_id) :
+  core_memory_layout_MemoryLayout_read_lemma π.
+Proof.
+  core_memory_layout_MemoryLayout_read_prelude.
+
+  repeat liRStep; liShow.
+  liInst Hevar1 (MemoryLayout_inv_t).
+  liInst Hevar2 Spin_ty.
   repeat liRStep; liShow.
 
   all: print_remaining_goal.
