verification/theories/memory_tracker/page_allocator/page_allocator_extra.v
@@ -1,0 +1,26 @@
+From refinedrust Require Import typing.
+From ace.theories.page Require Import page_extra.
+
+(** [m1] is a correct abstraction of [m2] to only specify the number of pages at a given size. *)
+Definition page_allocator_maps_related (m1 : gmap page_size nat) (m2 : gmap page_size (place_rfn (list (place_rfn page)))) : Prop :=
+  ∀ (sz : page_size) num_pages, m1 !! sz = Some num_pages →
+    ∃ list_pages : list page,
+      (* There exists a list of pages at that size *)
+      m2 !! sz = Some (# (<#> list_pages)) ∧
+      (* The length matches up *)
+      length list_pages = num_pages ∧
+      (* The pages have the right size *)
+      Forall (λ pg : page, pg.(page_sz) = sz) list_pages.
+
+(** The list of [pages] forms a contiguous region of memory, one page after another. *)
+Fixpoint pages_are_contiguous (pages : list page) : Prop :=
+  match pages with
+  | [] => True
+  | pg1 :: pgs =>
+      match pgs with
+      | [] => True
+      | pg2 :: pgs' =>
+          pages_are_contiguous pgs ∧
+          pg1.(page_loc) +ₗ (page_size_in_bytes_Z pg1.(page_sz)) = pg2.(page_loc)
+      end
+  end.
